System transition: IC Management Canister: Starting a canister [DONE]

theories/IC.thy
@@ -422,6 +422,10 @@ fun message_cycles :: "('b, 'p, 'uid, 'canid, 's, 'c, 'cid) message \<Rightarrow
 | "message_cycles (Func_message _ _ ep _) = cycles_reserved ep"
 | "message_cycles (Response_message orig _ ref_cycles) = carried_cycles orig + ref_cycles"
 
+fun status_cycles :: "('b, 'p, 'uid, 'canid, 's, 'c, 'cid) can_status \<Rightarrow> nat" where
+  "status_cycles (Stopping os) = sum_list (map (carried_cycles \<circ> fst) os) + sum_list (map snd os)"
+| "status_cycles _ = 0"
+
 lift_definition call_ctxt_carried_cycles :: "('p, 'uid, 'canid, 'b, 's, 'c, 'cid) call_ctxt \<Rightarrow> nat" is
   "\<lambda>ctxt. (if needs_to_respond ctxt
     then available_cycles ctxt + carried_cycles (origin ctxt)
@@ -442,7 +446,8 @@ definition total_cycles :: "('p, 'uid, 'canid, 'b, 'w, 'sm, 'c, 's, 'cid, 'pk) i
     let cycles_in_balances = list_map_sum_vals id (balances ic) in
     let cycles_in_messages = sum_list (map message_cycles (messages ic)) in
     let cycles_in_contexts = list_map_sum_vals call_ctxt_carried_cycles (call_contexts ic) in
-    cycles_in_balances + cycles_in_messages + cycles_in_contexts)"
+    let cycles_in_statuses = list_map_sum_vals status_cycles (canister_status ic) in
+    cycles_in_balances + cycles_in_messages + cycles_in_contexts + cycles_in_statuses)"
 
 (* Accessor functions *)
 
@@ -948,7 +953,7 @@ proof -
   show ?thesis
     using assms
     by (auto simp: ic_canister_creation_pre_def ic_canister_creation_post_def total_cycles_def Let_def msgs
-        list_map_sum_out[where ?g=id] split: message.splits option.splits)
+        list_map_sum_out[where ?g=id] list_map_sum_out[where ?g=status_cycles] split: message.splits option.splits)
 qed
 
 
@@ -1292,7 +1297,100 @@ proof -
   show ?thesis
     using assms
     by (auto simp: ic_canister_deletion_pre_def ic_canister_deletion_post_def ic_canister_deletion_lost_cycles_def total_cycles_def call_ctxt_carried_cycles cid_def Let_def msgs
-        list_map_del_sum[where ?g=id and ?f="balances S"] split: message.splits option.splits sum.splits)
+        list_map_del_sum[where ?g=id and ?f="balances S"] list_map_del_sum[where ?g=status_cycles and ?f="canister_status S"]
+        split: message.splits option.splits sum.splits)
+qed
+
+
+
+(* System transition: IC Management Canister: Starting a canister (not stopping) [DONE] *)
+
+definition ic_canister_start_not_stopping_pre :: "nat \<Rightarrow> ('p, 'uid, 'canid, 'b, 'tr, 'w, 'sm, 'c, 's, 'cid, 'pk) ic \<Rightarrow> bool" where
+  "ic_canister_start_not_stopping_pre n S = (n < length (messages S) \<and> (case messages S ! n of Call_message orig cer cee mn d trans_cycles q \<Rightarrow>
+    (q = Unordered \<or> (\<forall>j < n. message_queue (messages S ! j) \<noteq> Some q)) \<and>
+    cee = ic_principal \<and>
+    mn = encode_string ''start_canister'' \<and>
+    (case candid_parse_cid d of Some cid \<Rightarrow>
+    (case (list_map_get (canister_status S) cid, list_map_get (controllers S) cid) of (Some can_status, Some ctrls) \<Rightarrow>
+      (can_status = Running \<or> can_status = Stopped) \<and> cer \<in> ctrls
+    | _ \<Rightarrow> False) | _ \<Rightarrow> False)
+  | _ \<Rightarrow> False))"
+
+definition ic_canister_start_not_stopping_post :: "nat \<Rightarrow> ('p, 'uid, 'canid, 'b, 'tr, 'w, 'sm, 'c, 's, 'cid, 'pk) ic \<Rightarrow> ('p, 'uid, 'canid, 'b, 'tr, 'w, 'sm, 'c, 's, 'cid, 'pk) ic" where
+  "ic_canister_start_not_stopping_post n S = (case messages S ! n of Call_message orig cer cee mn d trans_cycles q \<Rightarrow>
+    let cid = the (candid_parse_cid d) in
+    S\<lparr>canister_status := list_map_set (canister_status S) cid Running,
+      messages := take n (messages S) @ drop (Suc n) (messages S) @ [Response_message orig (Reply (blob_of_candid Candid_empty)) trans_cycles]\<rparr>)"
+
+lemma ic_canister_start_not_stopping_cycles_inv:
+  assumes "ic_canister_start_not_stopping_pre n S"
+  shows "total_cycles S = total_cycles (ic_canister_start_not_stopping_post n S)"
+proof -
+  obtain orig cer cee mn d trans_cycles q cid where msg: "messages S ! n = Call_message orig cer cee mn d trans_cycles q"
+    and cid_def: "candid_parse_cid d = Some cid"
+    using assms
+    by (auto simp: ic_canister_start_not_stopping_pre_def split: message.splits option.splits)
+  define older where "older = take n (messages S)"
+  define younger where "younger = drop (Suc n) (messages S)"
+  have msgs: "messages S = older @ Call_message orig cer cee mn d trans_cycles q # younger" "(older @ w # younger) ! n = w"
+    "take n older = older" "take (n - length older) ws = []" "drop (Suc n) older = []"
+    "drop (Suc n - length older) (w # ws) = ws" for w ws
+    using id_take_nth_drop[of n "messages S"] assms
+    by (auto simp: ic_canister_start_not_stopping_pre_def msg younger_def older_def nth_append)
+  show ?thesis
+    using assms
+    by (auto simp: ic_canister_start_not_stopping_pre_def ic_canister_start_not_stopping_post_def total_cycles_def call_ctxt_carried_cycles cid_def Let_def msgs
+        list_map_sum_in[where ?g=status_cycles] split: message.splits option.splits sum.splits)
+qed
+
+
+
+(* System transition: IC Management Canister: Starting a canister (stopping) [DONE] *)
+
+definition ic_canister_start_stopping_pre :: "nat \<Rightarrow> ('p, 'uid, 'canid, 'b, 'tr, 'w, 'sm, 'c, 's, 'cid, 'pk) ic \<Rightarrow> bool" where
+  "ic_canister_start_stopping_pre n S = (n < length (messages S) \<and> (case messages S ! n of Call_message orig cer cee mn d trans_cycles q \<Rightarrow>
+    (q = Unordered \<or> (\<forall>j < n. message_queue (messages S ! j) \<noteq> Some q)) \<and>
+    cee = ic_principal \<and>
+    mn = encode_string ''start_canister'' \<and>
+    (case candid_parse_cid d of Some cid \<Rightarrow>
+    (case (list_map_get (canister_status S) cid, list_map_get (controllers S) cid) of (Some (Stopping _), Some ctrls) \<Rightarrow>
+      cer \<in> ctrls
+    | _ \<Rightarrow> False) | _ \<Rightarrow> False)
+  | _ \<Rightarrow> False))"
+
+definition ic_canister_start_stopping_post :: "nat \<Rightarrow> ('p, 'uid, 'canid, 'b, 'tr, 'w, 'sm, 'c, 's, 'cid, 'pk) ic \<Rightarrow> ('p, 'uid, 'canid, 'b, 'tr, 'w, 'sm, 'c, 's, 'cid, 'pk) ic" where
+  "ic_canister_start_stopping_post n S = (case messages S ! n of Call_message orig cer cee mn d trans_cycles q \<Rightarrow>
+    let cid = the (candid_parse_cid d);
+    orig_cycles_to_msg = (\<lambda>(or, cyc). Response_message or (response.Reject CANISTER_REJECT (encode_string ''Canister has been restarted'')) cyc) in
+    (case list_map_get (canister_status S) cid of Some (Stopping os) \<Rightarrow>
+    S\<lparr>canister_status := list_map_set (canister_status S) cid Running,
+      messages := take n (messages S) @ drop (Suc n) (messages S) @ [Response_message orig (Reply (blob_of_candid Candid_empty)) trans_cycles] @
+      map orig_cycles_to_msg os\<rparr>))"
+
+lemma ic_canister_start_stopping_cycles_inv:
+  assumes "ic_canister_start_stopping_pre n S"
+  shows "total_cycles S = total_cycles (ic_canister_start_stopping_post n S)"
+proof -
+  obtain orig cer cee mn d trans_cycles q cid where msg: "messages S ! n = Call_message orig cer cee mn d trans_cycles q"
+    and cid_def: "candid_parse_cid d = Some cid"
+    using assms
+    by (auto simp: ic_canister_start_stopping_pre_def split: message.splits option.splits)
+  define older where "older = take n (messages S)"
+  define younger where "younger = drop (Suc n) (messages S)"
+  have msgs: "messages S = older @ Call_message orig cer cee mn d trans_cycles q # younger" "(older @ w # younger) ! n = w"
+    "take n older = older" "take (n - length older) ws = []" "drop (Suc n) older = []"
+    "drop (Suc n - length older) (w # ws) = ws" for w ws
+    using id_take_nth_drop[of n "messages S"] assms
+    by (auto simp: ic_canister_start_stopping_pre_def msg younger_def older_def nth_append)
+  have F1: "(message_cycles \<circ> (\<lambda>(or, y). Response_message or (response.Reject CANISTER_REJECT (encode_string ''Canister has been restarted'')) y)) = (\<lambda>(or, y). carried_cycles or + y)"
+    by auto
+  have F2: "(\<Sum>(or, y)\<leftarrow>xs. carried_cycles or + y) = sum_list (map (carried_cycles \<circ> fst) xs) + sum_list (map snd xs)" for xs
+    by (induction xs) auto
+  show ?thesis
+    using assms list_map_sum_in_ge[where ?g=status_cycles and ?f="canister_status S" and ?x=cid]
+    by (auto simp: ic_canister_start_stopping_pre_def ic_canister_start_stopping_post_def total_cycles_def call_ctxt_carried_cycles cid_def Let_def msgs F1 F2
+        list_map_sum_in[where ?g=status_cycles and ?f="canister_status S"]
+        split: message.splits option.splits sum.splits can_status.splits)
 qed
 
 
@@ -1396,6 +1494,8 @@ export_code request_submission_pre request_submission_post
   ic_code_upgrade_pre ic_code_upgrade_post
   ic_code_uninstallation_pre ic_code_uninstallation_post
   ic_canister_deletion_pre ic_canister_deletion_post
+  ic_canister_start_not_stopping_pre ic_canister_start_not_stopping_post
+  ic_canister_start_stopping_pre ic_canister_start_stopping_post
   ic_depositing_cycles_pre ic_depositing_cycles_post
   ic_random_numbers_pre ic_random_numbers_post
 in Haskell module_name IC file_prefix code
